More progress on allocate_dtyp_spec_fin_inf.
- Expose uvalue_sbyte in FinByte module.
- Lemmas about generate_undef_bytes between fin / inf memory (as well
   as other helpers)
- Getting further along in allocate_dtyp_spec_fin_inf with the
  MemPropT_fin_inf_bind lemma, trying to make sure that it's sensible.

src/coq/Handlers/MemoryModules/FiniteSizeof.v
@@ -141,7 +141,8 @@ Inductive UByte (uvalue : Type) :=
 | mkUByte (uv : uvalue) (dt : dtyp) (idx : uvalue) (sid : store_id) : UByte uvalue.
 
 Module FinByte (ADDR : MemoryAddress.ADDRESS) (IP : MemoryAddress.INTPTR) (SIZEOF : Sizeof) (LLVMEvents:LLVM_INTERACTIONS(ADDR)(IP)(SIZEOF)) : ByteImpl(ADDR)(IP)(SIZEOF)(LLVMEvents)
-with  Definition SByte := UByte LLVMEvents.DV.uvalue.
+with  Definition SByte := UByte LLVMEvents.DV.uvalue
+with  Definition uvalue_sbyte := mkUByte LLVMEvents.DV.uvalue.
   Import LLVMEvents.
   Import DV.
 
